Wavelet/Compile/Prog/Simulation.lean
@@ -574,9 +574,9 @@ private theorem aop_interp_map_inj
   | interp_forward h₁ h₂ =>
     simp [Vector.toList_map, hinputs', houtputs']
     exact .interp_forward (by simp [h₁]) (by simp [h₂])
-  | interp_fork h₁ =>
+  | interp_fork h₁ h₂ =>
     simp [Vector.toList_map, hinputs', houtputs']
-    exact .interp_fork (by simp [h₁])
+    exact .interp_fork (by simp [h₁]) (by simp [h₂])
   | interp_const h₁ =>
     simp [Vector.toList_map, hinputs', houtputs']
     exact .interp_const (by simp [h₁])
